[minor] Refactor notions of memory update.

pico-ifc-coq/dyn_allocation/Concrete.v
@@ -160,18 +160,24 @@ Inductive cache_hit_read (m: list Atom) : Z -> Z -> Prop :=
                      (TAG_ResPC: tag_in_mem m addrTagResPC (Vint tagrpc)),
                 cache_hit_read m tagr tagrpc.
 
+Definition user_memory_doesnt_change (m m' : memory) :=
+  forall b, Mem.stamp b = User -> Mem.get_frame m' b = Mem.get_frame m b.
+
+Definition kernel_memory_extension (m m' : memory) : Prop :=
+  forall b fr,
+    Mem.stamp b = Kernel ->
+    b <> cblock ->
+    Mem.get_frame m b = Some fr ->
+    Mem.get_frame m' b = Some fr.
+
 (** [fault_handler_memory_update] expresses the changes to the memory
 that the fault handler is allowed to do. This means that the user
 memory doesn't change and that all kernel blocks that were already
 present stay untouched, with the possible exception of the cache block *)
 
 Definition fault_handler_memory_update (m m': memory) :=
-  forall b,
-    (Mem.stamp b = User -> Mem.get_frame m' b = Mem.get_frame m b) /\
-    (forall fr, Mem.stamp b = Kernel ->
-                b <> cblock ->
-                Mem.get_frame m b = Some fr ->
-                Mem.get_frame m' b = Some fr).
+  user_memory_doesnt_change m m' /\
+  kernel_memory_extension m m'.
 
 Definition update_cache_spec_mvec (m m': memory) :=
   fault_handler_memory_update m m' /\
