pico-ifc-coq/dyn_allocation/FaultRoutine.v
@@ -1157,10 +1157,10 @@ Proof.
   clear - Hm' Hm'' stamp_cblock.
   split.
   - split.
-    + intros USER.
+    + intros b USER.
       transitivity (Mem.get_frame m' b);
       eapply get_frame_store_neq; eauto; congruence.
-    + intros fr _ NEQ DEF.
+    + intros b fr _ NEQ DEF.
       rewrite <- DEF.
       transitivity (Mem.get_frame m' b);
       eapply get_frame_store_neq; eauto.
